src/bbcache/BitBlastingCCacheCorrect.v
@@ -61,7 +61,7 @@ Proof.
       apply (bit_blast_srem_correct Hbb) |
       apply (bit_blast_smod_correct Hbb) |
       apply (bit_blast_shl_correct Hszgt0 Hsize Hbb) |
-      apply (bit_blast_lshr_correct Hbb) |
+      apply (bit_blast_lshr_correct Hszgt0 Hsize Hbb) |
       apply (bit_blast_ashr_correct Hbb) |
       apply (bit_blast_concat_correct Hbb) ];
     done.
